Simplify Forward Analysis.

theories/AnalysisForward.v
@@ -9,7 +9,7 @@ Set Implicit Arguments.
 
 Definition forwardF (sT:stmt) (Dom:stmt->Type) `{BoundedSemiLattice (Dom sT)}
            (forward:〔params〕 ->
-                    forall s (ST:subTerm s sT) (a:ann (Dom sT)), ann (Dom sT) * 〔Dom sT〕)
+                    forall s (ST:subTerm s sT) (d:Dom sT) (a:ann (Dom sT)), ann (Dom sT) * 〔Dom sT〕)
            (ZL:list params)
            (F:list (params * stmt)) (anF:list (ann (Dom sT)))
            (ST:forall n s, get F n s -> subTerm (snd s) sT)
@@ -21,13 +21,11 @@ Definition forwardF (sT:stmt) (Dom:stmt->Type) `{BoundedSemiLattice (Dom sT)}
   - destruct anF as [|a anF'].
     + eapply nil.
     + econstructor 2.
-      * refine (forward ZL (snd Zs) _ a).
+      * refine (forward ZL (snd Zs) _ (getAnn a) a).
         eapply (ST 0 Zs); eauto using get.
       * eapply (g F' anF').
         eauto using get.
 Defined.
-
-
 
 Arguments forwardF [sT] [Dom] {H} {H0} forward ZL F anF ST : clear implicits.
 
@@ -56,43 +54,43 @@ Fixpoint forward (sT:stmt) (Dom: stmt -> Type) `{BoundedSemiLattice (Dom sT)}
            (ftransform :
               forall sT, list params ->
                     forall s, subTerm s sT -> Dom sT -> anni (Dom sT))
-           (ZL:list (params)) (st:stmt) (ST:subTerm st sT) (a:ann (Dom sT)) {struct st}
+           (ZL:list (params)) (st:stmt) (ST:subTerm st sT) (d:Dom sT) (a:ann (Dom sT)) {struct st}
   :  ann (Dom sT) * list (Dom sT)
   := match st as st', a return st = st' -> ann (Dom sT) * list (Dom sT) with
-    | stmtLet x e s as st, ann1 d ans =>
+    | stmtLet x e s as st, ann1 _ ans =>
       fun EQ =>
         let an := ftransform sT ZL st ST d in
         let (ans', AL) := forward Dom ftransform ZL (subTerm_EQ_Let EQ ST)
-                                 (setTopAnn ans (getAnni d an)) in
+                                 (getAnni d an) ans in
         (ann1 d ans', AL)
-    | stmtIf x s t, ann2 d ans ant =>
+    | stmtIf x s t, ann2 _ ans ant =>
       fun EQ =>
         let an := ftransform sT ZL st ST d in
         let (ans', AL) := forward Dom ftransform ZL (subTerm_EQ_If1 EQ ST)
-                                 (setTopAnn ans (getAnniLeft d an)) in
+                                 (getAnniLeft d an) ans in
         let (ant', AL') := forward Dom ftransform ZL (subTerm_EQ_If2 EQ ST)
-                                  (setTopAnn ant (getAnniRight d an)) in
+                                  (getAnniRight d an) ant in
         (ann2 d ans' ant', zip join AL AL')
-    | stmtApp f Y as st, ann0 d as an =>
+    | stmtApp f Y as st, ann0 _ as an =>
       fun EQ =>
         let an := ftransform sT ZL st ST d in
         (ann0 d, list_update_at ((fun _ => bottom) ⊝ ZL) (counted f) (getAnni d an))
 
 
-    | stmtReturn x as st, ann0 d as an =>
+    | stmtReturn x as st, ann0 _ as an =>
       fun EQ => (ann0 d, (fun _ => bottom) ⊝ ZL)
 
-    | stmtFun F t as st, annF d anF ant =>
+    | stmtFun F t as st, annF _ anF ant =>
       fun EQ =>
         let ZL' := List.map fst F ++ ZL in
         let (ant', ALt) := forward Dom ftransform ZL' (subTerm_EQ_Fun1 EQ ST)
-                                  (setTopAnn ant d) in
+                                  d ant in
         let anF' := forwardF (forward Dom ftransform) ZL' F anF
                             (subTerm_EQ_Fun2 EQ ST) in
         let AL' := fold_left (zip join) (snd ⊝ anF') ALt in
         (annF d (zip (@setTopAnn _) (fst ⊝ anF') AL') ant',
          drop ❬F❭ AL')
-    | _, an => fun EQ => (an, (fun _ => bottom) ⊝ ZL)
+    | _, an => fun EQ => (ann0 d, (fun _ => bottom) ⊝ ZL)
   end eq_refl.
 
 Lemma fold_list_length A B (f:list B -> (list A * bool) -> list B) (a:list (list A * bool)) (b: list B)
@@ -109,7 +107,7 @@ Qed.
 
 Lemma forwardF_get  (sT:stmt) (Dom:stmt->Type) `{BoundedSemiLattice (Dom sT)}
            (forward:〔params〕 ->
-                     forall s (ST:subTerm s sT) (a:ann (Dom sT)),
+                     forall s (ST:subTerm s sT) (d:Dom sT) (a:ann (Dom sT)),
                        ann (Dom sT) * list (Dom sT))
            (ZL:list params)
            (F:list (params * stmt)) (anF:list (ann (Dom sT)))
@@ -118,7 +116,7 @@ Lemma forwardF_get  (sT:stmt) (Dom:stmt->Type) `{BoundedSemiLattice (Dom sT)}
       :
         { Zs : params * stmt & {GetF : get F n Zs &
         { a : ann (Dom sT) & { getAnF : get anF n a &
-        { ST' : subTerm (snd Zs) sT | aa = forward ZL (snd Zs) ST' a
+        { ST' : subTerm (snd Zs) sT | aa = forward ZL (snd Zs) ST' (getAnn a) a
         } } } } }.
 Proof.
   eapply get_getT in GetBW.
@@ -130,14 +128,14 @@ Qed.
 
 Lemma get_forwardF  (sT:stmt) (Dom:stmt->Type) `{BoundedSemiLattice (Dom sT)}
            (forward:〔params〕 ->
-                     forall s (ST:subTerm s sT) (a:ann (Dom sT)),
+                     forall s (ST:subTerm s sT) (d:Dom sT) (a:ann (Dom sT)),
                        ann (Dom sT) * list (Dom sT))
            (ZL:list params)
            (F:list (params * stmt)) (anF:list (ann (Dom sT)))
            (ST:forall n s, get F n s -> subTerm (snd s) sT) n Zs a
   :get F n Zs
    -> get anF n a
-   -> { ST' | get (forwardF forward ZL F anF ST) n (forward ZL (snd Zs) ST' a) }.
+   -> { ST' | get (forwardF forward ZL F anF ST) n (forward ZL (snd Zs) ST' (getAnn a) a) }.
 Proof.
   intros GetF GetAnF.
   eapply get_getT in GetF.
@@ -175,7 +173,7 @@ Lemma forward_length (sT:stmt) (Dom : stmt -> Type) `{BoundedSemiLattice (Dom sT
       (f: forall sT, list params ->
                 forall s, subTerm s sT -> Dom sT -> anni (Dom sT))
   : forall (s : stmt) (ST:subTerm s sT) (ZL:list params),
-    forall a : ann (Dom sT), ❬snd (forward Dom f ZL ST a)❭ = ❬ZL❭.
+    forall d (a : ann (Dom sT)), ❬snd (forward Dom f ZL ST d a)❭ = ❬ZL❭.
 Proof.
   sind s; destruct s; destruct a; simpl; eauto with len;
     repeat let_pair_case_eq; subst; simpl in *; eauto.
@@ -194,7 +192,7 @@ Lemma forward_length_ass
       (f: forall sT, list params ->
                 forall s, subTerm s sT -> Dom sT -> anni (Dom sT))
   : forall (s : stmt) (ST:subTerm s sT) (ZL:list params) k,
-    forall a : ann (Dom sT), ❬ZL❭ = k -> ❬snd (forward Dom f ZL ST a)❭ = k.
+    forall d (a : ann (Dom sT)), ❬ZL❭ = k -> ❬snd (forward Dom f ZL ST d a)❭ = k.
 Proof.
   intros. rewrite forward_length; eauto.
 Qed.
@@ -204,7 +202,7 @@ Lemma forward_length_le_ass
       (f: forall sT, list params ->
                 forall s, subTerm s sT -> Dom sT -> anni (Dom sT))
   : forall (s : stmt) (ST:subTerm s sT) (ZL:list params) k,
-    forall a : ann (Dom sT), ❬ZL❭ <= k -> ❬snd (forward Dom f ZL ST a)❭ <= k.
+    forall d (a : ann (Dom sT)), ❬ZL❭ <= k -> ❬snd (forward Dom f ZL ST d a)❭ <= k.
 Proof.
   intros. rewrite forward_length; eauto.
 Qed.
@@ -214,7 +212,7 @@ Lemma forward_length_le_ass_right
       (f: forall sT, list params ->
                 forall s, subTerm s sT -> Dom sT -> anni (Dom sT))
   : forall (s : stmt) (ST:subTerm s sT) (ZL:list params) k,
-    forall a : ann (Dom sT), k <= ❬ZL❭ -> k <= ❬snd (forward Dom f ZL ST a)❭.
+    forall d (a : ann (Dom sT)), k <= ❬ZL❭ -> k <= ❬snd (forward Dom f ZL ST d a)❭.
 Proof.
   intros. rewrite forward_length; eauto.
 Qed.
@@ -225,10 +223,10 @@ Hint Resolve @forward_length_ass forward_length_le_ass forward_length_le_ass_rig
 Lemma forward_annotation sT (Dom:stmt->Type) `{BoundedSemiLattice (Dom sT)} s
       (f: forall sT, list params ->
                 forall s, subTerm s sT -> Dom sT -> anni (Dom sT))
-  : forall ZL a (ST:subTerm s sT), annotation s a
-               -> annotation s (fst (forward Dom f ZL ST a)).
+  : forall ZL d a (ST:subTerm s sT), annotation s a
+               -> annotation s (fst (forward Dom f ZL ST d a)).
 Proof.
-  sind s; intros ZL a ST Ann; destruct s; inv Ann; simpl;
+  sind s; intros ZL d a ST Ann; destruct s; inv Ann; simpl;
     repeat let_pair_case_eq; subst; eauto 20 using @annotation, setTopAnn_annotation.
   - econstructor; eauto using setTopAnn_annotation.
     + rewrite zip_length. rewrite map_length.
@@ -242,24 +240,36 @@ Proof.
       eauto using setTopAnn_annotation, setAnn_annotation.
 Qed.
 
-Lemma forward_getAnn (sT:stmt) (Dom : stmt -> Type) `{BoundedSemiLattice (Dom sT)}
-      (f: forall sT, list params ->
-                forall s, subTerm s sT -> Dom sT -> anni (Dom sT)) s (ST:subTerm s sT) ZL a an
-  : ann_R eq (fst (@forward sT Dom _ _ f ZL s ST (setTopAnn an a))) an
-    -> getAnn an = a.
-Proof.
-  intros. destruct s, an; inv H1; simpl in *; eauto;
-  repeat let_case_eq; repeat simpl_pair_eqs; subst; simpl in *; inv H2; eauto.
-Qed.
-
 Lemma forward_getAnn' (sT:stmt) (Dom : stmt -> Type) `{BoundedSemiLattice (Dom sT)}
       (f: forall sT, list params ->
-                forall s, subTerm s sT -> Dom sT -> anni (Dom sT)) s (ST:subTerm s sT) ZL an
-  : getAnn (fst (@forward sT Dom _ _ f ZL s ST an)) = getAnn an.
+                forall s, subTerm s sT -> Dom sT -> anni (Dom sT)) s (ST:subTerm s sT) ZL d an
+  : getAnn (fst (@forward sT Dom _ _ f ZL s ST d an)) = d.
 Proof.
   intros. destruct s, an; simpl in *; eauto;
   repeat let_pair_case_eq; simpl; eauto.
 Qed.
+
+Lemma forward_getAnn (sT:stmt) (Dom : stmt -> Type) `{BoundedSemiLattice (Dom sT)}
+      (f: forall sT, list params ->
+                forall s, subTerm s sT -> Dom sT -> anni (Dom sT)) s (ST:subTerm s sT) ZL a an
+  : ann_R eq (fst (@forward sT Dom _ _ f ZL s ST a an)) an
+    -> getAnn an = a.
+Proof.
+  intros. eapply ann_R_get in H1.
+  rewrite forward_getAnn' in H1. eauto.
+Qed.
+
+
+Ltac simpl_forward_setTopAnn :=
+  repeat match goal with
+         | [H : ann_R eq (fst (forward ?unreachable_code_transform ?ZL
+                                       ?s ?ST ?a ?sa)) ?sa |- _ ] =>
+           let X := fresh "H" in
+           match goal with
+           | [ H' : getAnn sa = a |- _ ] => fail 1
+           | _ => exploit (forward_getAnn _ _ _ _ _ H) as X
+           end
+         end; subst; try eassumption.
 
 Ltac fold_po :=
   repeat match goal with
@@ -277,28 +287,28 @@ Lemma forward_monotone (sT:stmt) (Dom : stmt -> Type) `{BoundedSemiLattice (Dom 
       (fMon:forall s (ST ST':subTerm s sT) ZL,
           forall a b, a ⊑ b -> f sT ZL s ST a ⊑ f sT ZL s ST' b)
   : forall (s : stmt) (ST ST':subTerm s sT) (ZL:list params),
-    forall a b : ann (Dom sT), annotation s a ->  a ⊑ b ->
-                           forward Dom f ZL ST a ⊑ forward Dom f ZL ST' b.
-Proof with eauto using setTopAnn_annotation, poLe_setTopAnn, poLe_getAnni.
+    forall (d d' : Dom sT) (a b : ann (Dom sT)), d ⊑ d' -> a ⊑ b ->
+                           forward Dom f ZL ST d a ⊑ forward Dom f ZL ST' d' b.
+Proof with eauto using poLe_setTopAnn, poLe_getAnni.
   intros s.
-  sind s; destruct s; intros ST ST' ZL d d' Ann LE; simpl forward; inv LE; inv Ann;
-    simpl forward; repeat let_pair_case_eq; subst; eauto 10 using @ann_R.
+  sind s; destruct s; intros ST ST' ZL d d' a b LE_d LE; simpl forward; inv LE;
+    simpl forward; repeat let_pair_case_eq; subst; eauto 10 using @ann_R;
+      try now (econstructor; simpl; eauto using @ann_R).
   - econstructor; simpl; eauto; fold_po.
     + econstructor; eauto; fold_po.
-      eapply IH; eauto using setTopAnn_annotation, poLe_setTopAnn, poLe_getAnni.
-    + eapply IH; eauto using setTopAnn_annotation, poLe_setTopAnn, poLe_getAnni.
+      eapply IH; eauto using poLe_getAnni.
+    + eapply IH; eauto using poLe_getAnni.
   - econstructor; simpl; eauto.
     + econstructor; eauto.
-      eapply (IH s1); eauto using setTopAnn_annotation, poLe_setTopAnn, poLe_getAnniLeft.
-      eapply (IH s2); eauto using setTopAnn_annotation, poLe_setTopAnn, poLe_getAnniRight.
+      eapply (IH s1); eauto using poLe_getAnniLeft.
+      eapply (IH s2); eauto using poLe_getAnniRight.
     +
       eapply PIR2_ojoin_zip.
-      * eapply IH; eauto using setTopAnn_annotation, poLe_setTopAnn, poLe_getAnniLeft.
-      * eapply IH; eauto using setTopAnn_annotation, poLe_setTopAnn, poLe_getAnniRight.
-  - econstructor; eauto. simpl.
+      * eapply IH; eauto using poLe_getAnniLeft.
+      * eapply IH; eauto using poLe_getAnniRight.
+  - econstructor; eauto. simpl. econstructor; eauto.
     eapply update_at_poLe.
     eapply poLe_getAnni; eauto.
-  - econstructor; simpl; eauto.
   - fold_po.
     assert (forall (n : nat) (x x' : ann (Dom sT) * 〔Dom sT〕),
                get (forwardF (forward Dom f) (fst ⊝ F ++ ZL) F ans
@@ -307,6 +317,9 @@ Proof with eauto using setTopAnn_annotation, poLe_setTopAnn, poLe_getAnni.
                              (subTerm_EQ_Fun2 eq_refl ST')) n x' ->
                x ⊑ x'). {
       intros; inv_get; dcr; eauto.
+      eapply IH; eauto.
+      exploit H3; eauto.
+      eapply ann_R_get; eauto.
     }
     econstructor; simpl; eauto.
     + econstructor; eauto.
@@ -323,26 +336,24 @@ Proof with eauto using setTopAnn_annotation, poLe_setTopAnn, poLe_getAnni.
         inv_zip H6; clear H6. inv_map H8; clear H8.
         inv_zip H7; clear H7. inv_map H8; clear H8.
         exploit H5; eauto.
-        exploit get_PIR2; [ eapply PIR2_fold_zip_join | eapply H10 | eapply H13 | ].
-        eapply PIR2_get. intros. inv_map H14; clear H14. inv_map H15; clear H15.
+        exploit get_PIR2; [ eapply PIR2_fold_zip_join | eapply H9 | eapply H10 | ].
+        eapply PIR2_get. intros. inv_map H12; clear H12. inv_map H11; clear H11.
         eapply H5; eauto.
         repeat rewrite map_length.
         repeat rewrite forwardF_length.
         repeat rewrite forward_length. rewrite H2; reflexivity.
-        eapply IH; eauto using setTopAnn_annotation.
+        eapply IH; eauto.
         eapply ann_R_setTopAnn; eauto.
-        eapply ann_R_setTopAnn; eauto. eapply H8.
-      * eapply IH; eauto using setTopAnn_annotation.
-        eapply ann_R_setTopAnn; eauto.
+        eapply H8.
+      * eapply IH; eauto.
     + eapply PIR2_drop. eapply PIR2_fold_zip_join.
       * eapply PIR2_get; eauto.
         intros. inv_map H6. inv_map H7.
-        exploit H5; eauto. eapply H13.
+        exploit H5; eauto. eapply H10.
         repeat rewrite map_length.
         repeat rewrite forwardF_length.
         repeat rewrite forward_length. rewrite H2; reflexivity.
-      * eapply IH; eauto using setTopAnn_annotation.
-        eapply ann_R_setTopAnn; eauto.
+      * eapply IH; eauto.
 Qed.
 
 Require Import FiniteFixpointIteration.
@@ -360,21 +371,20 @@ Instance makeForwardAnalysis (Dom:stmt -> Type)
   {
     step := fun X : {a : ann (Dom s) | annotation s a} =>
                       exist (fun a0 : ann (Dom s) => annotation s a0)
-                            (fst (forward Dom f nil (subTerm_refl _) (setTopAnn (proj1_sig X) i)))
-                                 (forward_annotation Dom f nil (subTerm_refl _) _);
+                            (fst (forward Dom f nil (subTerm_refl _) i (proj1_sig X)))
+                                 (forward_annotation Dom f nil i (subTerm_refl _) _);
     initial_value :=
       exist (fun a : ann (Dom s) => annotation s a)
             (setAnn bottom s)
             (setAnn_annotation bottom s)
   }.
 Proof.
-  - destruct X. eapply setTopAnn_annotation; eauto.
+  - destruct X; eauto.
   - intros [d Ann]; simpl.
     pose proof (@ann_bottom s (Dom s) _ _ _ Ann).
     eapply H0.
   - intros. eapply terminating_sig.
     eapply terminating_ann. eauto.
   - intros [a Ann] [b Bnn] LE; simpl in *.
-    eapply (forward_monotone Dom f (fMon s)); eauto using setTopAnn_annotation.
-    eapply ann_R_setTopAnn; eauto.
+    eapply (forward_monotone Dom f (fMon s)); eauto.
 Defined.
